LambdaS5/coq/LjsPrettyRulesIndexed.v
@@ -234,102 +234,92 @@ Inductive red_exprh : nat -> ctx -> store -> ext_expr -> out -> Prop :=
     red_exprh k c st (expr_set_obj_attr_2 oa v1 o) o
 
 (* get_field *)
-| red_exprh_get_field : forall k c st e1 e2 e3 o o',
+| red_exprh_get_field : forall k c st e1 e2 o o',
     red_exprh k c st e1 o ->
-    red_exprh k c st (expr_get_field_1 o e2 e3) o' ->
-    red_exprh (S k) c st (expr_get_field e1 e2 e3) o'
-| red_exprh_get_field_1 : forall k c st' st v1 e2 e3 o o',
+    red_exprh k c st (expr_get_field_1 o e2) o' ->
+    red_exprh (S k) c st (expr_get_field e1 e2) o'
+| red_exprh_get_field_1 : forall k c st' st v1 e2 o o',
     red_exprh k c st e2 o ->
-    red_exprh k c st (expr_get_field_2 v1 o e3) o' ->
-    red_exprh k c st' (expr_get_field_1 (out_ter st (res_value v1)) e2 e3) o'
-| red_exprh_get_field_1_abort : forall k c st e2 e3 o,
+    red_exprh k c st (expr_get_field_2 v1 o) o' ->
+    red_exprh k c st' (expr_get_field_1 (out_ter st (res_value v1)) e2) o'
+| red_exprh_get_field_1_abort : forall k c st e2 o,
     abort o ->
-    red_exprh k c st (expr_get_field_1 o e2 e3) o
-| red_exprh_get_field_2 : forall k c st' st v1 v2 e3 o o',
-    red_exprh k c st e3 o ->
-    red_exprh k c st (expr_get_field_3 v1 v2 o) o' ->
-    red_exprh k c st' (expr_get_field_2 v1 (out_ter st (res_value v2)) e3) o'
-| red_exprh_get_field_2_abort : forall k c st v1 e3 o,
-    abort o ->
-    red_exprh k c st (expr_get_field_2 v1 o e3) o
-| red_exprh_get_field_3 : forall k c st' st v3 ptr s oattr o,
+    red_exprh k c st (expr_get_field_1 o e2) o
+| red_exprh_get_field_2 : forall k c st' st ptr s oattr o,
     get_property st ptr s = result_some oattr ->
-    red_exprh k c st (expr_get_field_4 ptr oattr v3) o ->
-    red_exprh k c st' (expr_get_field_3 (value_object ptr) (value_string s) (out_ter st (res_value v3))) o
-| red_exprh_get_field_3_abort : forall k c st v1 v2 o,
+    red_exprh k c st (expr_get_field_3 ptr oattr) o ->
+    red_exprh k c st' (expr_get_field_2 (value_object ptr) (out_ter st (res_value (value_string s)))) o
+| red_exprh_get_field_2_abort : forall k c st v1 o,
     abort o ->
-    red_exprh k c st (expr_get_field_3 v1 v2 o) o
-| red_exprh_get_field_4_no_field : forall k c st ptr v3,
-    red_exprh k c st (expr_get_field_4 ptr None v3) (out_ter st (res_value value_undefined))
-| red_exprh_get_field_4_get_field : forall k c st ptr v3 data,
-    red_exprh k c st (expr_get_field_4 ptr (Some (attributes_data_of data)) v3) (out_ter st (res_value (attributes_data_value data)))
-| red_exprh_get_field_4_getter : forall k c st ptr v3 acc o,
-    red_exprh k c st (expr_app_2 (attributes_accessor_get acc) [v3; value_object ptr] nil) o ->
-    red_exprh k c st (expr_get_field_4 ptr (Some (attributes_accessor_of acc)) v3) o
+    red_exprh k c st (expr_get_field_2 v1 o) o
+| red_exprh_get_field_3_no_field : forall k c st ptr,
+    red_exprh k c st (expr_get_field_3 ptr None) (out_ter st (res_value value_undefined))
+| red_exprh_get_field_3_get_field : forall k c st ptr data,
+    red_exprh k c st (expr_get_field_3 ptr (Some (attributes_data_of data))) (out_ter st (res_value (attributes_data_value data)))
+| red_exprh_get_field_3_getter : forall k c st st' ptr v3 acc o,
+    (st', v3) = add_object st (default_object) ->
+    red_exprh k c st' (expr_app_2 (attributes_accessor_get acc) [v3; value_object ptr] nil) o ->
+    red_exprh k c st (expr_get_field_3 ptr (Some (attributes_accessor_of acc))) o
 
 (* set_field *)
-| red_exprh_set_field : forall k c st e1 e2 e3 e4 o o',
+| red_exprh_set_field : forall k c st e1 e2 e3 o o',
     red_exprh k c st e1 o ->
-    red_exprh k c st (expr_set_field_1 o e2 e3 e4) o' ->
-    red_exprh (S k) c st (expr_set_field e1 e2 e3 e4) o'
-| red_exprh_set_field_1 : forall k c st' st v1 e2 e3 e4 o o',
+    red_exprh k c st (expr_set_field_1 o e2 e3) o' ->
+    red_exprh (S k) c st (expr_set_field e1 e2 e3) o'
+| red_exprh_set_field_1 : forall k c st' st v1 e2 e3 o o',
     red_exprh k c st e2 o ->
-    red_exprh k c st (expr_set_field_2 v1 o e3 e4) o' ->
-    red_exprh k c st' (expr_set_field_1 (out_ter st (res_value v1)) e2 e3 e4) o'
+    red_exprh k c st (expr_set_field_2 v1 o e3) o' ->
+    red_exprh k c st' (expr_set_field_1 (out_ter st (res_value v1)) e2 e3) o'
 | red_exprh_set_field_1_abort : forall k c st e2 e3 e4 o,
     abort o ->
-    red_exprh k c st (expr_set_field_1 o e2 e3 e4) o
-| red_exprh_set_field_2 : forall k c st' st v1 v2 e3 e4 o o',
+    red_exprh k c st (expr_set_field_1 o e2 e3) o
+| red_exprh_set_field_2 : forall k c st' st v1 v2 e3 o o',
     red_exprh k c st e3 o ->
-    red_exprh k c st (expr_set_field_3 v1 v2 o e4) o' ->
-    red_exprh k c st' (expr_set_field_2 v1 (out_ter st (res_value v2)) e3 e4) o'
-| red_exprh_set_field_2_abort : forall k c st v1 e3 e4 o,
+    red_exprh k c st (expr_set_field_3 v1 v2 o) o' ->
+    red_exprh k c st' (expr_set_field_2 v1 (out_ter st (res_value v2)) e3) o'
+| red_exprh_set_field_2_abort : forall k c st v1 e3 o,
     abort o ->
-    red_exprh k c st (expr_set_field_2 v1 o e3 e4) o
-| red_exprh_set_field_3 : forall k c st' st v1 v2 v3 e4 o o',
-    red_exprh k c st e4 o ->
-    red_exprh k c st (expr_set_field_4 v1 v2 v3 o) o' ->
-    red_exprh k c st' (expr_set_field_3 v1 v2 (out_ter st (res_value v3)) e4) o'
-| red_exprh_set_field_3_abort : forall k c st v1 v2 e4 o,
-    abort o ->
-    red_exprh k c st (expr_set_field_3 v1 v2 o e4) o
-| red_exprh_set_field_4 : forall k c st' st ptr obj oattr s v3 v4 o,
+    red_exprh k c st (expr_set_field_2 v1 o e3) o
+| red_exprh_set_field_3 : forall k c st' st ptr obj oattr s v3 v4 o,
     get_property st ptr s = result_some oattr ->
     get_object st ptr = Some obj ->
-    red_exprh k c st (expr_set_field_5 ptr obj oattr s v3 v4) o ->
-    red_exprh k c st' (expr_set_field_4 (value_object ptr) (value_string s) v3 (out_ter st (res_value v4))) o
-| red_exprh_set_field_4_abort : forall k c st v1 v2 v3 o,
+    red_exprh k c st (expr_set_field_4 ptr obj oattr s v3) o ->
+    red_exprh k c st' (expr_set_field_3 (value_object ptr) (value_string s) (out_ter st (res_value v3))) o
+| red_exprh_set_field_3_abort : forall k c st v1 v2 o,
     abort o ->
-    red_exprh k c st (expr_set_field_4 v1 v2 v3 o) o
-| red_exprh_set_field_5_set_field : forall k c st st1 ptr obj data s v3 v4,
+    red_exprh k c st (expr_set_field_3 v1 v2 o) o
+| red_exprh_set_field_4_set_field : forall k c st st1 ptr obj data s v3,
     get_object_property obj s <> None ->
     attributes_data_writable data = true ->
     st1 = update_object st ptr (set_object_property obj s (attributes_data_of (attributes_data_value_update data v3))) ->
-    red_exprh k c st (expr_set_field_5 ptr obj (Some (attributes_data_of data)) s v3 v4) (out_ter st1 (res_value v3))
-| red_exprh_set_field_5_shadow_field : forall k c st st1 ptr obj data s v3 v4,
+    red_exprh k c st (expr_set_field_4 ptr obj (Some (attributes_data_of data)) s v3) (out_ter st1 (res_value v3))
+| red_exprh_set_field_4_shadow_field : forall k c st st1 ptr obj data s v3,
     get_object_property obj s = None ->
     object_extensible obj = true ->
     attributes_data_writable data = true ->
     st1 = update_object st ptr (set_object_property obj s (attributes_data_of (attributes_data_intro v3 true true true))) ->
-    red_exprh k c st (expr_set_field_5 ptr obj (Some (attributes_data_of data)) s v3 v4) (out_ter st1 (res_value v3))
-| red_exprh_set_field_5_add_field : forall k c st st1 ptr obj s v3 v4,
+    red_exprh k c st (expr_set_field_4 ptr obj (Some (attributes_data_of data)) s v3) (out_ter st1 (res_value v3))
+| red_exprh_set_field_4_add_field : forall k c st st1 ptr obj s v3,
     object_extensible obj = true ->
     st1 = update_object st ptr (set_object_property obj s (attributes_data_of (attributes_data_intro v3 true true true))) ->
-    red_exprh k c st (expr_set_field_5 ptr obj None s v3 v4) (out_ter st1 (res_value v3))
-| red_exprh_set_field_5_setter : forall k c st ptr obj acc s v3 v4 o,
-    red_exprh k c st (expr_app_2 (attributes_accessor_set acc) [v4; value_object ptr] nil) o ->
-    red_exprh k c st (expr_set_field_5 ptr obj (Some (attributes_accessor_of acc)) s v3 v4) o
-| red_exprh_set_field_5_unwritable : forall k c st ptr obj data s v3 v4,
+    red_exprh k c st (expr_set_field_4 ptr obj None s v3) (out_ter st1 (res_value v3))
+| red_exprh_set_field_4_setter : forall k c st st' ptr obj acc s v3 v4 o,
+    (st', v4) = add_object st (object_with_properties 
+                      (Heap.write Heap.empty "0" (attributes_data_of 
+                        (attributes_data_intro v3 true false false))) default_object) ->
+    red_exprh k c st' (expr_app_2 (attributes_accessor_set acc) [v4; value_object ptr] nil) o ->
+    red_exprh k c st (expr_set_field_4 ptr obj (Some (attributes_accessor_of acc)) s v3) o
+| red_exprh_set_field_4_unwritable : forall k c st ptr obj data s v3,
     attributes_data_writable data = false ->
-    red_exprh k c st (expr_set_field_5 ptr obj (Some (attributes_data_of data)) s v3 v4) (out_ter st (res_exception (value_string "unwritable-field")))
-| red_exprh_set_field_5_unextensible_add : forall k c st ptr obj s v3 v4,
+    red_exprh k c st (expr_set_field_4 ptr obj (Some (attributes_data_of data)) s v3) (out_ter st (res_exception (value_string "unwritable-field")))
+| red_exprh_set_field_4_unextensible_add : forall k c st ptr obj s v3,
     object_extensible obj = false ->
-    red_exprh k c st (expr_set_field_5 ptr obj None s v3 v4) (out_ter st (res_value value_undefined))
-| red_exprh_set_field_5_unextensible_shadow : forall k c st ptr obj data s v3 v4,
+    red_exprh k c st (expr_set_field_4 ptr obj None s v3) (out_ter st (res_value value_undefined))
+| red_exprh_set_field_4_unextensible_shadow : forall k c st ptr obj data s v3,
     attributes_data_writable data = true ->
     get_object_property obj s = None ->
     object_extensible obj = false ->
-    red_exprh k c st (expr_set_field_5 ptr obj (Some (attributes_data_of data)) s v3 v4) (out_ter st (res_value value_undefined))
+    red_exprh k c st (expr_set_field_4 ptr obj (Some (attributes_data_of data)) s v3) (out_ter st (res_value value_undefined))
 
 (* delete_field *)
 | red_exprh_delete_field : forall k c st e1 e2 o o',
